Update Debugvarproof

backend/Debugvarproof.v
@@ -302,12 +302,6 @@ Lemma senv_preserved:
   Senv.equiv ge tge.
 Proof (Genv.senv_match TRANSF).
 
-Lemma genv_next_preserved:
-  Genv.genv_next tge = Genv.genv_next ge.
-Proof.
-  apply senv_preserved.
-Qed.
-
 Lemma functions_translated:
   forall (v: val) (f: fundef),
   Genv.find_funct ge v = Some f ->
@@ -337,9 +331,9 @@ Lemma find_function_translated:
   forall ros ls f b,
   find_block ge ros ls = Some b ->
   Genv.find_funct_ptr ge b = Some f ->
-  exists tb tf,
-    find_block tge ros ls = Some tb /\
-    Genv.find_funct_ptr tge tb = Some tf /\
+  exists tf,
+    find_block tge ros ls = Some b /\
+    Genv.find_funct_ptr tge b = Some tf /\
     transf_fundef f = OK tf.
 Proof.
   unfold find_block; intros; destruct ros; simpl.
@@ -361,13 +355,9 @@ Proof.
   exists (Val.longofwords v1 v2); auto with barg.
 Qed.
 
-Section WITHINITLS.
-
-Variable init_ls: locset.
-
 Lemma eval_add_delta_ranges:
   forall s f sp c rs m before after,
-  star (step init_ls) tge (State s f sp (add_delta_ranges before after c) rs m)
+  star step tge (State s f sp (add_delta_ranges before after c) rs m)
              E0 (State s f sp c rs m).
 Proof.
   intros. unfold add_delta_ranges.
@@ -394,6 +384,9 @@ Qed.
 (** Matching between program states. *)
 
 Inductive match_stackframes: Linear.stackframe -> Linear.stackframe -> Prop :=
+  | match_stackframe_parent:
+      forall rs,
+      match_stackframes (Parent rs) (Parent rs)
   | match_stackframe_intro:
       forall f sp rs c tf tc before after,
       match_function f tf ->
@@ -411,13 +404,13 @@ Inductive match_states: Linear.state ->  Linear.state -> Prop :=
       match_states (State s f sp c rs m)
                    (State ts tf sp tc rs m)
   | match_states_call:
-      forall s f rs m tf ts b tb
+      forall s f rs m tf ts b
         (FIND: Genv.find_funct_ptr ge b = Some f)
-        (TFIND: Genv.find_funct_ptr tge tb = Some tf),
+        (TFIND: Genv.find_funct_ptr tge b = Some tf),
       list_forall2 match_stackframes s ts ->
       transf_fundef f = OK tf ->
       match_states (Callstate s b rs m)
-                   (Callstate ts tb rs m)
+                   (Callstate ts b rs m)
   | match_states_return:
       forall s rs m ts,
       list_forall2 match_stackframes s ts ->
@@ -427,7 +420,7 @@ Inductive match_states: Linear.state ->  Linear.state -> Prop :=
 Lemma parent_locset_match:
   forall s ts,
   list_forall2 match_stackframes s ts ->
-  parent_locset init_ls ts = parent_locset init_ls s.
+  parent_locset ts = parent_locset s.
 Proof.
   induction 1; simpl. auto. inv H; auto.
 Qed.
@@ -435,13 +428,11 @@ Qed.
 (** The simulation diagram. *)
 
 Theorem transf_step_correct:
-  forall s1 t s2, step init_ls ge s1 t s2 ->
+  forall s1 t s2, step ge s1 t s2 ->
   forall ts1 (MS: match_states s1 ts1),
-  exists w, (exists t', match_events_query _ w t t') /\
-  forall t', match_events cc_id w t t' ->
-  exists ts2, plus (step init_ls) tge ts1 t' ts2 /\ match_states s2 ts2.
+  exists ts2, plus step tge ts1 t ts2 /\ match_states s2 ts2.
 Proof.
-  induction 1; intros ts1 MS; stable_step; inv MS; try (inv TRC).
+  induction 1; intros ts1 MS; inv MS; try (inv TRC).
 - (* getstack *)
   econstructor; split.
   eapply plus_left. constructor; auto. apply eval_add_delta_ranges. traceEq.
@@ -474,13 +465,13 @@ Proof.
   apply eval_add_delta_ranges. traceEq.
   constructor; auto.
 - (* call *)
-  exploit find_function_translated; eauto. intros (tb' & tf' & FB & A & B).
+  exploit find_function_translated; eauto. intros (tf' & FB & A & B).
   econstructor; split.
   apply plus_one.
-  econstructor. eexact FB. eexact A. symmetry; apply sig_preserved; auto. traceEq.
+  econstructor. exact FB. eexact A. symmetry; apply sig_preserved; auto. traceEq.
   econstructor; eauto. constructor; auto. constructor; auto.
 - (* tailcall *)
-  exploit find_function_translated; eauto. intros (tb' & tf' & FB & A & B).
+  exploit find_function_translated; eauto. intros (tf' & FB & A & B).
   exploit parent_locset_match; eauto. intros PLS.
   econstructor; split.
   apply plus_one.
@@ -545,36 +536,62 @@ Proof.
   constructor; auto.
 Qed.
 
-End WITHINITLS.
-
 Lemma transf_initial_states:
-  forall st1, initial_state prog st1 ->
-  exists st2, initial_state tprog st2 /\ match_states st1 st2.
+  forall w q1 q2, match_query cc_id w q1 q2 ->
+  forall st1, initial_state ge q1 st1 ->
+  exists st2, initial_state tge q2 st2 /\ match_states st1 st2.
 Proof.
-  intros. inversion H.
+  intros [ ] q _ [ ].
+  intros. inv H.
   exploit function_ptr_translated; eauto. intros [tf [A B]].
-  exists (Callstate nil b (Locmap.init Vundef) m0); split.
-  econstructor; eauto. eapply (Genv.init_mem_transf_partial TRANSF); eauto.
-  rewrite (match_program_main TRANSF), symbols_preserved. auto.
-  rewrite <- H3. apply sig_preserved. auto.
-  econstructor; eauto. constructor.
+  replace (fn_sig f) with (funsig tf) by auto using (sig_preserved (Internal f) tf).
+  exists (Callstate (Parent rs :: nil) (Block.glob id) rs m); split.
+  - monadInv B. econstructor; eauto.
+  - econstructor; eauto. repeat constructor.
+Qed.
+
+Lemma transf_external:
+  forall st1 st2 q1,
+    match_states st1 st2 ->
+    at_external ge st1 q1 ->
+    exists w q2,
+      match_query cc_id w q1 q2 /\
+      at_external tge st2 q2 /\
+      forall r1 r2 st1',
+        match_reply cc_id w r1 r2 ->
+        after_external ge st1 r1 st1' ->
+        exists st2',
+          after_external tge st2 r2 st2' /\
+          match_states st1' st2'.
+Proof.
+  intros st1 st2 q Hst Hq.
+  exists tt, q. intuition auto.
+  - constructor.
+  - destruct Hq. inv Hst.
+    apply function_ptr_translated in H as (f' & Hf' & H). monadInv H.
+    econstructor; eauto.
+  - destruct Hq. inv Hst. inv H0. inv H.
+    eexists. split; constructor; auto.
 Qed.
 
 Lemma transf_final_states:
-  forall st1 st2 r,
-  match_states st1 st2 -> final_state st1 r -> final_state st2 r.
+  forall w st1 st2 r1,
+  match_states st1 st2 -> final_state st1 r1 ->
+  exists r2, match_reply cc_id w r1 r2 /\ final_state st2 r2.
 Proof.
-  intros. inv H0. inv H. inv H5. econstructor; eauto.
+  intros. inv H0. inv H. inv H4. inv H1.
+  exists (rs, m). split; constructor.
 Qed.
 
 Theorem transf_program_correct:
-  forward_simulation cc_id (semantics prog) (semantics tprog).
+  forward_simulation cc_id cc_id (semantics prog) (semantics tprog).
 Proof.
-  eapply forward_simulation_plus.
+  eapply forward_simulation_plus with (match_states := fun _ => match_states).
   apply senv_preserved.
   eexact transf_initial_states.
+  intros _. eexact transf_external.
   eexact transf_final_states.
-  apply transf_step_correct.
+  intros _. apply transf_step_correct.
 Qed.
 
 End PRESERVATION.
